MirrorCharge!/src/MirrorCharge/Java/Reify.v
@@ -1,0 +1,156 @@
+Require Import MirrorCore.Reify.Reify.
+Require Import MirrorCore.Lambda.Expr.
+
+Require Import MirrorCharge.Java.Syntax.
+
+Require Import Charge.Open.Stack.
+Require Import Charge.Open.Subst.
+Require Import Charge.Open.OpenILogic.
+
+Require Import Java.Logic.AssertionLogic.
+Require Import Java.Logic.SpecLogic.
+Require Import Java.Language.Program.
+Require Import Java.Language.Lang.
+Require Import Java.Semantics.OperationalSemantics.
+
+Reify Declare Patterns patterns_imp_typ := Syntax.typ.
+
+Reify Declare Patterns patterns_imp := (ExprCore.expr Syntax.typ Syntax.func).
+
+Reify Declare Syntax reify_imp_typ :=
+  { (@Patterns.CPatterns Syntax.typ patterns_imp_typ
+     (@Patterns.CFail Syntax.typ))
+  }.
+
+Definition eval2 (e : dexpr) : stack -> val := eval e.
+
+Reify Declare Typed Table term_table : BinNums.positive => reify_imp_typ.
+
+Let Ext x := @ExprCore.Inj Syntax.typ Syntax.func (inl (inl x)).
+
+Reify Declare Syntax reify_imp :=
+  { (@Patterns.CPatterns _ patterns_imp
+    (@Patterns.CApp _ (@ExprCore.App Syntax.typ Syntax.func)
+    (@Patterns.CAbs _ reify_imp_typ (@ExprCore.Abs Syntax.typ Syntax.func)
+    (@Patterns.CVar _ (@ExprCore.Var Syntax.typ Syntax.func)
+    (@Patterns.CTypedTable _ _ _ term_table Ext
+    (@Patterns.CFail (ExprCore.expr Syntax.typ Syntax.func)))))))
+  }.
+
+Let _Inj := @ExprCore.Inj Syntax.typ Syntax.func.
+
+Local Notation "x @ y" := (@RApp x y) (only parsing, at level 30).
+Local Notation "'!!' x" := (@RExact _ x) (only parsing, at level 25).
+Local Notation "'?' n" := (@RGet n RIgnore) (only parsing, at level 25).
+Local Notation "'?!' n" := (@RGet n RConst) (only parsing, at level 25).
+Local Notation "'#'" := RIgnore (only parsing, at level 0).
+
+Reify Pattern patterns_imp_typ += (@RImpl (?0) (?1)) => (fun (a b : function reify_imp_typ) => tyArr a b).
+
+Reify Pattern patterns_imp_typ += (!! asn)  => tyAsn.
+Reify Pattern patterns_imp_typ += (!! sasn) => tySasn.
+Reify Pattern patterns_imp_typ += (!! (@vlogic String.string _)) => tyPure.
+Reify Pattern patterns_imp_typ += (!! Prop) => tyProp.
+Reify Pattern patterns_imp_typ += (!! spec) => tySpec.
+
+Reify Pattern patterns_imp_typ += (!! (@list String.string)) => tyVarList.
+Reify Pattern patterns_imp_typ += (!! (@list (@Open.expr (Lang.var) SVal))) => tyVarList.
+Reify Pattern patterns_imp_typ += (!! (@list (Lang.var * @Open.expr (Lang.var) SVal))) => tySubstList.
+Reify Pattern patterns_imp_typ += (!! nat) => tyNat.
+Reify Pattern patterns_imp_typ += (!! sval) => tyVal.
+Reify Pattern patterns_imp_typ += (!! String.string) => tyString.
+Reify Pattern patterns_imp_typ += (!! Prog_wf) => tyProg.
+Reify Pattern patterns_imp_typ += (!! stack) => tyStack.
+Reify Pattern patterns_imp_typ += (!! cmd) => tyCmd.
+Reify Pattern patterns_imp_typ += (!! SS.t) => tyFields.
+Reify Pattern patterns_imp_typ += (!! dexpr) => tyExpr.
+Reify Pattern patterns_imp_typ += (!! @Subst.subst (Lang.var) SVal) => tySubst.
+
+Reify Pattern patterns_imp_typ += (!! Fun @ ?0 @ ?1) => (fun (a b : function reify_imp_typ) => tyArr a b).
+
+Reify Pattern patterns_imp += (RHasType String.string (?!0)) => (fun (s : id String.string) => mkString [s] : expr typ func).
+Reify Pattern patterns_imp += (RHasType field (?!0)) => (fun (f : id field) => mkString [f] : expr typ func).
+Reify Pattern patterns_imp += (RHasType Lang.var (?!0)) => (fun (f : id Lang.var) => mkString [f] : expr typ func).
+Reify Pattern patterns_imp += (RHasType sval (?!0)) => (fun (v : id sval) => mkVal [v] : expr typ func).
+Reify Pattern patterns_imp += (RHasType cmd (?!0)) => (fun (c : id cmd) => mkCmd [c] : expr typ func).
+Reify Pattern patterns_imp += (RHasType dexpr (?!0)) => (fun (e : id dexpr) => mkExpr [e] : expr typ func).
+
+Reify Pattern patterns_imp += (!! (@eq) @ ?0) => (fun (x : function reify_imp_typ) => fEq [x] : expr typ func).
+
+(** Intuitionistic Operators **)
+Reify Pattern patterns_imp += (!! @ILogic.lentails @ ?0 @ #) => (fun (x : function reify_imp_typ) => fEntails [x] : expr typ func).
+Reify Pattern patterns_imp += (!! @ILogic.ltrue @ ?0 @ #) => (fun (x : function reify_imp_typ) => mkTrue [x] : expr typ func).
+Reify Pattern patterns_imp += (!! @ILogic.lfalse @ ?0 @ #) => (fun (x : function reify_imp_typ) => mkFalse [x] : expr typ func).
+Reify Pattern patterns_imp += (!! @ILogic.land @ ?0 @ #) => (fun (x : function reify_imp_typ) => fAnd [x] : expr typ func).
+Reify Pattern patterns_imp += (!! @ILogic.lor @ ?0 @ #) => (fun (x : function reify_imp_typ) => fOr [x] : expr typ func).
+Reify Pattern patterns_imp += (!! @ILogic.limpl @ ?0 @ #) => (fun (x : function reify_imp_typ) => fImpl [x] : expr typ func).
+Reify Pattern patterns_imp += (!! @ILogic.lexists @ ?0 @ # @ ?1) => (fun (x y : function reify_imp_typ) => fExists [x, y] : expr typ func).
+Reify Pattern patterns_imp += (!! @ILogic.lforall @ ?0 @ # @ ?1) => (fun (x y : function reify_imp_typ) => fForall [x, y] : expr typ func).
+
+(** Embedding Operators **)
+Reify Pattern patterns_imp += (!! @ILEmbed.embed @ ?0 @ ?1 @ #) => (fun (x y : function reify_imp_typ) => fEmbed [x, y] : expr typ func).
+
+(** Special cases for Coq's primitives **)
+Reify Pattern patterns_imp += (!! True) => (mkTrue [tyProp] : expr typ func).
+Reify Pattern patterns_imp += (!! False) => (mkFalse [tyProp] : expr typ func).
+Reify Pattern patterns_imp += (!! and) => (fAnd [tyProp] : expr typ func).
+Reify Pattern patterns_imp += (!! or) => (fOr [tyProp] : expr typ func).
+Reify Pattern patterns_imp += (RPi (?0) (?1)) => (fun (x : function reify_imp_typ) (y : function reify_imp) =>
+                                                   ExprCore.App (fForall [tyProp, x]) (ExprCore.Abs x y)).
+Reify Pattern patterns_imp += (RImpl (?0) (?1)) => (fun (x y : function reify_imp) => ExprCore.App (ExprCore.App (fImpl [tyProp]) x) y).
+
+(** Separation Logic Operators **)
+Reify Pattern patterns_imp += (!! @BILogic.sepSP @ ?0 @ #) => (fun (x : function reify_imp_typ) => (fStar [x] : expr typ func)).
+Reify Pattern patterns_imp += (!! @BILogic.empSP @ ?0 @ #) => (fun (x : function reify_imp_typ) => (mkEmp [x] : expr typ func)).
+
+(** Program Logic **)
+
+Reify Pattern patterns_imp += (!! triple) => (fTriple : expr typ func).
+Reify Pattern patterns_imp += (!! eval2) => (fEval : expr typ func).
+Reify Pattern patterns_imp += (!! stack_get) => (fStackGet : expr typ func).
+Reify Pattern patterns_imp += (!! stack_add) => (fStackSet : expr typ func).
+
+Reify Pattern patterns_imp += (!! pointsto) => (fPointsto : expr typ func).
+Check @pointsto.
+Reify Pattern patterns_imp += (!! @apply_subst @ (RHasType String.string (#)) @ # @ ?0) => (fun (x : function reify_imp_typ) => (fApplySubst [x]) : expr typ func).
+Reify Pattern patterns_imp += (!! @subst1 @(RHasType String.string (#)) @ # @ #) => (fSingleSubst : expr typ func).
+
+(** Applicative **)
+Reify Pattern patterns_imp += (!! @Applicative.ap @ !! (Fun stack) @ # @ ?0 @ ?1) => (fun (x y : function reify_imp_typ) => fAp [x, y] : expr typ func).
+Reify Pattern patterns_imp += (!! @Applicative.pure @ !! (Fun stack) @ # @ ?0) => (fun (x : function reify_imp_typ) => fConst [x] : expr typ func).
+(*
+(** Table Entries **)
+Local Notation "a >> b" := (tyArr a b) (at level 31,right associativity).
+
+Reify Seed Typed Table term_table += 1 => [ (tyLProp >> tyCmd >> tyLProp >> tySProp) , triple ].
+Reify Seed Typed Table term_table += 2 => [ (tyCmd >> tyCmd >> tyCmd) , Seq ].
+Reify Seed Typed Table term_table += 3 => [ (tyVariable >> tyExpr >> tyCmd) , Assign ].
+Reify Seed Typed Table term_table += 4 => [ (tyVariable >> tyExpr >> tyCmd) , Read ].
+Reify Seed Typed Table term_table += 5 => [ (tyExpr >> tyExpr >> tyCmd) , Write ].
+Reify Seed Typed Table term_table += 6 => [ tyCmd , Skip ].
+Reify Seed Typed Table term_table += 7 => [ (tyNat >> tyNat >> tyHProp) , PtsTo ].
+Reify Seed Typed Table term_table += 8 => [ (tyVariable >> (tyNat >> tyLProp) >> (tyNat >> tyLProp) >> tySProp) , function_spec ].
+*)
+Let elem_ctor : forall x : Syntax.typ, (forall ts : list Type, typD ts x) -> @SymEnv.function _ _ :=
+  @SymEnv.F _ _.
+
+Ltac reify_imp e :=
+  let k fs e :=
+      pose e in
+  reify_expr reify_imp k
+             [ (fun (y : @mk_dvar_map_abs _ _ _ (list Type) _ term_table elem_ctor) => True) ]
+             [ e ].
+
+Goal True.
+  reify_imp 1.
+  reify_imp (cseq cskip cskip).
+  reify_imp (ILogic.lentails True True).
+  reify_imp ((True -> False) -> True).
+  reify_imp (forall P Q, P /\ Q).
+  reify_imp (forall P : sasn, ILogic.lentails ILogic.ltrue P).
+  reify_imp (forall (G : spec) (P Q : sasn), ILogic.lentails G (triple P Q cskip)).
+  generalize (String.EmptyString : String.string).
+  intro x.
+  reify_imp (x = x).
+  exact I.
+Defined.
