MirrorCharge!/src/MirrorCharge/Java/Semantics.v
@@ -1,0 +1,77 @@
+Require Import Charge.Logics.ILogic.
+Require Import Charge.Logics.ILEmbed.
+Require Import Charge.Open.OpenILogic.
+Require Import Charge.Open.Subst.
+
+Require Import Java.Language.Lang.
+
+Require Import Java.Semantics.OperationalSemantics.
+Require Import Java.Semantics.AxiomaticSemantics.
+
+Require Import Java.Logic.SpecLogic.
+Require Import Java.Logic.AssertionLogic.
+
+Require Import ExtLib.Data.PreFun.
+Require Import ExtLib.Structures.Applicative.
+
+Require Import MirrorCharge.Java.Reify.
+Require Import MirrorCharge.Java.Syntax.
+
+Set Implicit Arguments.
+Set Strict Implicit.
+
+Local Instance Applicative_Fun A : Applicative (Fun A) :=
+{ pure := fun _ x _ => x
+; ap := fun _ _ f x y => (f y) (x y)
+}.
+
+Lemma rule_seq c1 c2 (P Q R : sasn) G
+      (Hc1 : G |-- {[P]} c1 {[Q]})
+      (Hc2 : G |-- {[Q]} c2 {[R]}) :
+  G |-- {[P]} cseq c1 c2 {[R]}.
+Proof.
+  apply rule_seq with Q; assumption.
+Qed.
+
+Lemma rule_skip P Q G : P |-- Q -> G |-- {[P]} cskip {[Q]}.
+Proof.
+  intros.
+  eapply roc_post; [eapply rule_skip | apply H].
+Qed.
+
+Lemma rule_if (e : dexpr) c1 c2 (P Q : sasn) G
+      (Hc1 : G |-- {[(@embed (@vlogic String.string _) sasn _ 
+      				  (ap (T := Fun stack)
+      				      (ap (pure (@eq sval)) (eval2 e)) 
+      				  (pure (vbool true)))) //\\ P]} c1 {[Q]})
+      (Hc2 : G |-- {[(@embed (@vlogic String.string _) sasn _ 
+      				  (ap (T := Fun stack)
+      				      (ap (pure (@eq sval)) (eval2 (E_not e))) 
+      				  (pure (vbool true)))) //\\ P]} c2 {[Q]}) :
+  G |-- {[P]} cif e c1 c2 {[Q]}.
+Proof.
+  eapply rule_if; unfold vlogic_eval, Open.liftn, Open.lift; simpl in *;
+  	[apply Hc1|apply Hc2].
+Qed.
+
+
+  Lemma rule_read_fwd (x y : String.string) (f : String.string) (e : dexpr) (P : sasn) (G : spec)
+    (HPT : P |-- ap (T := Fun stack) (ap (ap (pure pointsto) (stack_get y)) (pure f)) (eval2 e)) : 
+  (*  G |-- {[ P ]} 
+              cread x y f 
+              {[ Exists v : sval, (@embed (@vlogic String.string _) sasn _)
+    								      (ap (T := Fun stack) 
+    								          (ap (pure (@eq sval)) (stack_get x)) 
+    								          ((eval2 e)[{(pure v)//x}])) //\\ 
+    							   P[{(pure v)//x}]]}.*) True.
+  Proof.
+(*
+	reify_imp (stack_get y).
+	reify_imp (ap (T := Fun stack) (ap (ap (pure pointsto) (stack_get y)) (pure f)) (eval2 e)).
+	admit.
+	
+    simpl in *.
+    pose proof @rule_read_fwd x y f (eval2 e) P. unfold Open.liftn, Open.lift, open_eq, stack_get, Open.var_expr in *; simpl in *.
+	rewrite <- H; [apply ltrueR | apply HPT].
+	*)
+  Qed.
